Prove emulate and emulate_pctx well-typedness and simplify/automate some stuff here and there.

BackTrans/Emulate.v
@@ -38,25 +38,25 @@ Fixpoint emulate (n : nat) (t : U.UTm) : S.Tm :=
     | U.seq t₁ t₂ => S.seq (caseUnitUp n (emulate n t₁)) (emulate n t₂)
   end.
 
-Fixpoint emulate_pctx (n : nat) (t : U.PCtx) : S.PCtx :=
-  match t with
+Fixpoint emulate_pctx (n : nat) (C : U.PCtx) : S.PCtx :=
+  match C with
     | U.phole => S.phole
-    | U.pabs C => S.phole (* inArrDwn n (S.pabs (UVal n) (emulate_pctx n C)) *)
-    | U.papp₁ C t₂ => S.papp₁ S.phole (* (caseArrUp n (emulate_pctx n C)) *) (emulate n t₂)
+    | U.pabs C => S.pctx_cat (S.pabs (UVal n) (emulate_pctx n C)) (inArrDwn_pctx n)
+    | U.papp₁ C t₂ => S.papp₁ (S.pctx_cat (emulate_pctx n C) (caseArrUp_pctx n)) (emulate n t₂)
     | U.papp₂ t₁ C => S.papp₂ (caseArrUp n (emulate n t₁)) (emulate_pctx n C)
-    | U.pite₁ C₁ t₂ t₃ => S.pite₁ S.phole (* (caseBoolUp n (emulate_pctx n C₁)) *) (emulate n t₂) (emulate n t₃)
+    | U.pite₁ C₁ t₂ t₃ => S.pite₁ (S.pctx_cat (emulate_pctx n C₁) (caseBoolUp_pctx n)) (emulate n t₂) (emulate n t₃)
     | U.pite₂ t₁ C₂ t₃ => S.pite₂ (caseBoolUp n (emulate n t₁)) (emulate_pctx n C₂) (emulate n t₃)
     | U.pite₃ t₁ t₂ C₃ => S.pite₃ (caseBoolUp n (emulate n t₁)) (emulate n t₂) (emulate_pctx n C₃)
-    | U.ppair₁ C₁ t₂ => S.phole (* inProdDwn n (S.ppair₁ (emulate_pctx n C₁) (emulate n t₂)) *)
-    | U.ppair₂ t₁ C₂ => S.phole (* inProdDwn n (S.ppair₂ (emulate n t₁) (emulate_pctx n C₂)) *)
-    | U.pproj₁ C => S.phole (* S.pproj₁ (caseProdUp n (emulate_pctx n C)) *)
-    | U.pproj₂ C => S.phole (* S.pproj₂ (caseProdUp n (emulate_pctx n C)) *)
-    | U.pinl C => S.phole (* inSumDwn n (S.pinl (emulate_pctx n C)) *)
-    | U.pinr C => S.phole (* inSumDwn n (S.pinr (emulate_pctx n C)) *)
-    | U.pcaseof₁ C₁ t₂ t₃ => S.phole (* S.pcaseof₁ (caseSumUp n (emulate_pctx n C₁)) (emulate n t₂) (emulate n t₃) *)
+    | U.ppair₁ C₁ t₂ => S.pctx_cat (S.ppair₁ (emulate_pctx n C₁) (emulate n t₂)) (inProdDwn_pctx n)
+    | U.ppair₂ t₁ C₂ => S.pctx_cat (S.ppair₂ (emulate n t₁) (emulate_pctx n C₂)) (inProdDwn_pctx n) 
+    | U.pproj₁ C => S.pproj₁ (S.pctx_cat (emulate_pctx n C) (caseProdUp_pctx n))
+    | U.pproj₂ C => S.pproj₂ (S.pctx_cat (emulate_pctx n C) (caseProdUp_pctx n))
+    | U.pinl C => S.pctx_cat (S.pinl (emulate_pctx n C)) (inSumDwn_pctx n)
+    | U.pinr C => S.pctx_cat (S.pinr (emulate_pctx n C)) (inSumDwn_pctx n)
+    | U.pcaseof₁ C₁ t₂ t₃ => S.pcaseof₁ (S.pctx_cat (emulate_pctx n C₁) (caseSumUp_pctx n)) (emulate n t₂) (emulate n t₃)
     | U.pcaseof₂ t₁ C₂ t₃ => S.pcaseof₂ (caseSumUp n (emulate n t₁)) (emulate_pctx n C₂) (emulate n t₃)
     | U.pcaseof₃ t₁ t₂ C₃ => S.pcaseof₃ (caseSumUp n (emulate n t₁)) (emulate n t₂) (emulate_pctx n C₃)
-    | U.pseq₁ C₁ t₂ => S.phole (* S.seq (caseUnitUp n (emulate_pctx n C₁)) (emulate n t₂) *)
+    | U.pseq₁ C₁ t₂ => S.pseq₁ (S.pctx_cat (emulate_pctx n C₁) (caseUnitUp_pctx n)) (emulate n t₂)
     | U.pseq₂ t₁ C₂ => S.pseq₂ (caseUnitUp n (emulate n t₁)) (emulate_pctx n C₂)
   end.
 
@@ -76,7 +76,23 @@ Lemma emulate_T {n Γ t} :
   ⟨ Γ ⊢ t ⟩ →
   ⟪ toUVals n Γ ⊢ emulate n t : UVal n ⟫.
 Proof.
-  induction 1;
+  induction 1; unfold emulate;
   eauto using stlcOmegaT, toUVals_entry with typing uval_typing.
+Qed.
+
+Lemma emulate_T' {γ t n} :
+  ⟨ S γ ⊢ t ⟩ →
+  ⟪ toUVals n γ ▻ UVal n ⊢ emulate n t : UVal n ⟫.
+Proof.
+  change (toUVals n γ ▻ UVal n) with (toUVals n (S γ)).
+  eauto using emulate_T.
+Qed.
+
+Lemma emulate_pctx_T {n Γ Γ' C} :
+  ⟨ ⊢ C : Γ → Γ' ⟩ →
+  ⟪ ⊢ emulate_pctx n C : toUVals n Γ , UVal n → toUVals n Γ' , UVal n ⟫.
+Proof.
+  induction 1; unfold emulate_pctx;
+  eauto using toUVals_entry, inUnitDwn_pctx_T, inBoolDwn_pctx_T, inProdDwn_pctx_T, inSumDwn_pctx_T, inArrDwn_pctx_T, caseUnitUp_pctx_T, caseBoolUp_pctx_T, caseProdUp_pctx_T, caseSumUp_pctx_T, caseArrUp_pctx_T, emulate_T, emulate_T', PCtxTyping, caseSumUp_T with typing uval_typing.
 Qed.
 
